to prove that RenameTerm is total need a proofs of totality above functions

Yard.Core.Conversions.RenameTerm.fst
@@ -2,79 +2,58 @@ module Yard.Core.Conversions.RenameTerm
     open IL
     open Yard.Core.Conversions
 
-
 //--Переименование терминалов в нетерминалы в неподходящих правилах (вида s -> AB, s -> Ab, s -> bA)-------------------
-
-//TODO: infix operator? :(
 
     val isToken: elem 'a 'b -> Tot bool
     let isToken elem = match elem.rule with PToken _ -> true | _ -> false
 
     val isRef: elem 'a 'b -> Tot bool
     let isRef elem = match elem.rule with PRef(_,_) -> true | _ -> false
-
-    val isRefOpt: option (elem 'a 'b) -> Tot bool
-    let isRefOpt elemopt =
-        match elemopt with
-        | Some elem -> isRef elem
-        | None -> false
-
-
-//assume val instanceOf: a:Type -> Tot a
- 
-    assume val toTerminalRule: 
-        x:(Rule 'a 'b){
-            (fun x ->  
-                match x.body with
-                | PSeq(elements,_,_) -> List.length elements = 1 && isToken (List.Tot.hd elements) 
-                | _ -> false) 
-            x 
-        }
-    assume val toTwoNonTermRule: 
-        x:(Rule 'a 'b){
-            (fun x ->  
-                match x.body with
-                | PSeq(elements,_,_) -> List.length elements = 2 && isRefOpt (List.Tot.nth elements 0) && isRefOpt (List.Tot.nth elements 1)
-                | _ -> false) 
-            x 
-        }
-    //assume val startRule: 
-
+	
     val isCNF: Rule 'a 'b -> Tot bool
-    let isCNF (rule: Rule 'a 'b) = 
-        match rule with 
-        | toTerminalRule -> true
-        | toTwoNonTermRule -> true
-        | (x:(Rule 'a 'b){ (fun x -> match x.body with PSeq([],_,_) -> x.isStart | _ -> false) x }) -> true 
-        | _ -> false
-    
-    let renameTerm ruleList = 
+    let isCNF rule =
+        match rule.body with
+        | PSeq(elements,_,_) -> (List.Tot.length elements = 1) || 
+								(List.Tot.length elements = 2 && isRef (List.Tot.hd elements) && isRef (List.Tot.hd (List.Tot.tl elements))) ||
+								(List.Tot.length elements = 0 && rule.isStart)	
+        | _ -> false   
+		
+	val lengthBodyRule: Rule 'a 'b -> Tot int
+    let lengthBodyRule rule = List.length (match rule.body with PSeq(e, a, l) -> e | _ -> [])
+	
+	val renameRule: rule : (Rule 'a 'b){lengthBodyRule rule = 2} -> list (Rule 'a 'b) -> Tot (list (Rule 'a 'b))
+	let renameRule rule newRuleList = 		
+		let rename elem = 
+			if isToken elem then 
+				let newRuleName = new_Source0("new_" ^ (match elem.rule with PToken t -> t.text | _ -> "")) in 
+			
+				if (not (List.Tot.existsb (fun rl -> rl.name = newRuleName) newRuleList)) then
+					let newRule = TransformAux.createRule newRuleName rule.args (PSeq([elem], None, None)) false rule.metaArgs in 
+					(TransformAux.createSimpleElem (PRef(newRuleName, None)) elem.binding, [newRule])
+				else (TransformAux.createSimpleElem (PRef(newRuleName, None)) elem.binding, [])
+			else (elem, []) in 
+		
+		let elements = match rule.body with PSeq(e, _, _) -> e | x -> [] in
+		
+		let elem0 = rename (List.Tot.hd elements) in
+		let elem1 = rename (List.Tot.hd (List.Tot.tl elements)) in 
+		let elems = [fst elem0; fst elem1] in
+			
+		let renameElem = 
+			[{rule with body =
+			(match rule.body with
+			| PSeq(e, a, l) -> PSeq(elems, a, l)
+			| _ -> PSeq(elems, None, None) )}] in  
+		let newRuleEls =  List.Tot.append (snd elem0) (snd elem1) in 
+			List.Tot.append renameElem newRuleEls
+	
+	val renameTerm_acc: list (Rule 'a 'b) -> list (Rule 'a 'b) -> 
+						(Rule 'a 'b -> list (Rule 'a 'b) -> Tot (list (Rule 'a 'b)))
+						-> Tot (list (Rule 'a 'b)) 
+	let rec renameTerm_acc ruleList acc f =
+		match ruleList with 
+		| [] -> acc
+		| hd::tl -> renameTerm_acc tl (List.Tot.append acc (f hd acc)) f
 
-        []
-
-        (*
-        let newRuleList = ref [] in
-
-        let renameRule (rule: Rule _ _) = 
-
-            let rename (elem: elem _ _) = 
-                if isToken elem then 
-                    let newRuleName = new_Source0("new_" ^ (match elem.rule with PToken t -> t.text | _ -> "")) in 
-                    if (not (!newRuleList |> List.existsb (fun rl -> rl.name = newRuleName))) then
-                        let newRule = TransformAux.createRule newRuleName rule.args (PSeq([elem], None, None)) false rule.metaArgs in 
-                        newRuleList := !newRuleList @ [newRule];
-                    TransformAux.createSimpleElem (PRef(newRuleName, None)) elem.binding
-                else 
-                    elem in
-
-            let elements = match rule.body with PSeq(e, a, l) -> e | x -> [] in
-            let elems = [rename (List.nth elements 0); rename (List.nth elements 1)] in
-            [{rule with body =
-                (match rule.body with
-                | PSeq(e, a, l) -> elems, a, l
-                | _ -> elems, None, None)
-                    |> PSeq }] in
-        
-        in
-        (ruleList |> List.collect (fun rule -> if isCNF rule then [rule] else renameRule rule)) @ !newRuleList
-        *)
+	assume val renameTerm: list (Rule 'a 'b) -> Tot (list (Rule 'a 'b))
+	(* let renameTerm ruleList = renameTerm_acc ruleList [] (fun rule acc -> if isCNF rule then [rule] else renameRule rule acc) *)
